Weidenbach_Book/IsaSAT.thy
@@ -121,12 +121,12 @@ definition IsaSAT :: \<open>nat clause_l list \<Rightarrow> nat literal list opt
 definition extract_model_of_state_stat :: \<open>twl_st_wl_heur \<Rightarrow> nat literal list option \<times> stats\<close> where
   \<open>extract_model_of_state_stat U =
      (Some (map lit_of (get_trail_wl_heur U)),
-       (\<lambda>(M, _,  _, _, _ ,_ ,_ ,_, _, _, _, stat). stat) U)\<close>
+       (\<lambda>(M, _,  _, _, _ ,_ ,_ ,_, _, _, _, stat, _). stat) U)\<close>
 
 definition extract_state_stat :: \<open>twl_st_wl_heur \<Rightarrow> nat literal list option \<times> stats\<close> where
   \<open>extract_state_stat U =
      (None,
-       (\<lambda>(M, _, _, _, _ ,_ ,_ ,_, _, _, _, stat). stat) U)\<close>
+       (\<lambda>(M, _, _, _, _ ,_ ,_ ,_, _, _, _, stat, _). stat) U)\<close>
 
 definition empty_conflict :: \<open>nat literal list option\<close> where
   \<open>empty_conflict = Some []\<close>
@@ -353,10 +353,10 @@ declare cdcl_twl_stgy_prog_wl_D_code_ref'[to_hnr, OF refl, sepref_fr_rules]
 declare cdcl_twl_stgy_prog_wl_D_break_fast_code_ref'[to_hnr, OF refl, sepref_fr_rules]
 
 definition get_trail_wl_code :: \<open>twl_st_wll_trail \<Rightarrow> uint32 list option \<times> stats\<close> where
-  \<open>get_trail_wl_code = (\<lambda>((M, _), _, _, _, _ ,_ ,_ ,_, _, _, _, stat). (Some M, stat))\<close>
+  \<open>get_trail_wl_code = (\<lambda>((M, _), _, _, _, _ ,_ ,_ ,_, _, _, _, stat, _). (Some M, stat))\<close>
 
 definition get_stats_code :: \<open>twl_st_wll_trail \<Rightarrow> uint32 list option \<times> stats\<close> where
-  \<open>get_stats_code = (\<lambda>((M, _), _, _, _, _ ,_ ,_ ,_, _, _, _, stat). (None, stat))\<close>
+  \<open>get_stats_code = (\<lambda>((M, _), _, _, _, _ ,_ ,_ ,_, _, _, _, stat, _). (None, stat))\<close>
 
 
 definition (in -) model_stat_rel where
